#################################################################
###  Generated with the experimental alpha version of the TTL exporter of WebVOWL (version 1.1.3)  http://visualdataweb.de/webvowl/   ###
#################################################################

@prefix : 		<https://w3id.org/example> .
@prefix rdf: 		<http://www.w3.org/1999/02/22-rdf-syntax-ns#> .
@prefix rdfs: 		<http://www.w3.org/2000/01/rdf-schema#> .
@prefix owl: 		<http://www.w3.org/2002/07/owl#> .
@prefix xsd: 		<http://www.w3.org/2001/XMLSchema#> .
@prefix dc: 		<http://purl.org/dc/elements/1.1/#> .
@prefix xml: 		<http://www.w3.org/XML/1998/namespace> .
@base 			<https://w3id.org/example> .

<https://w3id.org/example> rdf:type owl:Ontology ;
                           dc:title "The example ontology"@en;
			            "Примерна онтология"@bg;
                           dc:description "This is an example ontology to illustrate some of the annotations that should be included"@en; 
                           owl:versionInfo "1.0.1"@en;
                           dc:creator "Daniel Garijo, Maria Poveda-Villalon" . 
#################################################################

###  Property Definitions (Number of Property) 4 ###
#  --------------------------- Property 0------------------------- 
<https://w3id.org/example#foundedIn> rdf:type owl:DatatypeProperty ;
                                     rdfs:comment "Date when an organization was founded" ;
                                     rdfs:label "foundedIn"@IRI-based; 
                                     rdfs:label "founded in"@en; 
                                     rdfs:domain <https://w3id.org/example#Organization>;
                                     rdfs:range xsd:date . 
#  --------------------------- Property 1------------------------- 
<https://w3id.org/example#partOf> rdf:type owl:ObjectProperty ;
                                  rdfs:comment "This property links instances from Researcher to Organization" ;
                                  rdfs:label "partOf"@IRI-based; 
                                  rdfs:label "part of"@en; 
                                  rdfs:domain <https://w3id.org/example#Researcher>;
                                  rdfs:range <https://w3id.org/example#Organization> . 
#  --------------------------- Property 2------------------------- 
<https://w3id.org/example#hasMentor> rdf:type owl:ObjectProperty ;
                                     rdfs:comment "This property links the students to the researcher who mentored them" ;
                                     rdfs:label "hasMentor"@IRI-based; 
                                     rdfs:label "has mentor"@en; 
                                     rdfs:domain <https://w3id.org/example#Student>;
                                     rdfs:range <https://w3id.org/example#Researcher> . 
#  --------------------------- Property 3------------------------- 
<https://w3id.org/example#hasMember> rdf:type owl:ObjectProperty ;
                                     rdfs:comment "This example property indicates that an Organization has a Researcher as member" ;
                                     rdfs:label "hasMember"@IRI-based; 
                                     rdfs:label "has member"@en; 
                                     rdfs:domain <https://w3id.org/example#Organization>;
                                     rdfs:range <https://w3id.org/example#Researcher> . 
###  Class Definitions (Number of Classes) 3 ###
#  --------------------------- Class  0------------------------- 
<https://w3id.org/example#Organization> rdf:type owl:Class; 
                                        rdfs:comment "An organized body of people with a particular purpose, especially a business, society, association, etc." ;
                                        rdfs:label "Organization"@IRI-based; 
                                        rdfs:label "Organization"@en . 
#  --------------------------- Class  1------------------------- 
<https://w3id.org/example#Student> rdf:type owl:Class; 
                                   rdfs:comment "Student is a class introduced in the version 1.0.1 of the ontology. " ;
                                   rdfs:label "Student"@IRI-based; 
                                   rdfs:label "Student"@en . 
#  --------------------------- Class  2------------------------- 
<https://w3id.org/example#Researcher> rdf:type owl:Class; 
                                      rdfs:comment "A definition of your class. For example, A researcher is a person who publishes scientific papers, writes research proposals and mentors students" ;
                                      rdfs:label "Researcher"@IRI-based; 
                                      rdfs:label "Researcher"@en .